src/Narcissus/Examples/Protobuf/ProtobufExtract.v
@@ -2,7 +2,7 @@ Require Import
         Coq.ZArith.BinInt
         ExtrOcamlBasic
         ExtrOcamlNatInt
-        ExtrOcamlZInt
+        (* ExtrOcamlZInt *)
         ExtrOcamlString.
 
 Require Import
@@ -22,6 +22,7 @@ Require Import
         (* Fiat.Narcissus.BinLib.AlignedDecoders *)
         Fiat.Narcissus.BinLib.AlignedMonads
         Fiat.Narcissus.Formats.WordOpt
+        Fiat.Narcissus.Formats.VarintOpt
         Fiat.Narcissus.Stores.EmptyStore
         Fiat.Narcissus.Examples.Protobuf.ProtobufSpec
         Fiat.Narcissus.Examples.Protobuf.ProtobufEncoder.
@@ -61,8 +62,6 @@ Extract Constant wzero => "(fun _ -> Int64.zero)".
 Extract Constant wzero' => "(fun _ -> Int64.zero)".
 Extract Constant wones => "(fun n -> Int64.sub (Int64.shift_left Int64.one n) Int64.one)".
 
-Extract Constant wordToN => "(fun _ w -> Int64.to_int w)". (* Not ideal *)
-
 Extract Constant SW_word => "(fun sz b n -> Int64.add (if b then Int64.shift_left Int64.one sz else Int64.zero) n)".
 
 Extract Inductive Word.word =>
@@ -79,13 +78,51 @@ Extract Constant rev => "List.rev".
 Extract Constant app => "List.append".
 Extract Constant length => "List.length".
 
-Extract Constant N.shiftl => "(lsl)".
-Extract Constant N.shiftr => "(lsr)".
-Extract Constant N.lor => "(lor)".
-Extract Constant N.land => "(land)".
-Extract Constant N.eqb => "(==)".
-Extract Constant N.eq_dec => "(==)".
+Extract Constant wordToN => "(fun _ w -> w)". (* Not ideal *)
+
+Extract Inductive positive => int64
+[ "(fun p->(Int64.add Int64.one (Int64.mul (Int64.of_int 2) p)))" "(fun p->(Int64.mul (Int64.of_int 2) p))" "Int64.one" ]
+"(fun f2p1 f2p f1 p ->
+   if p<=Int64.one then f1 () else if (Int64.rem p (Int64.of_int 2)) = Int64.zero then f2p (Int64.div p (Int64.of_int 2)) else f2p1 (Int64.div p (Int64.of_int 2)))".
+
+Extract Constant Pos.add => "Int64.add".
+Extract Constant Pos.succ => "Int64.succ".
+Extract Constant Pos.pred => "fun n -> Pervasives.max Int64.zero (Int64.sub n Int64.one)".
+Extract Constant Pos.sub => "fun n m -> Pervasives.max Int64.zero (Int64.sub n m)".
+Extract Constant Pos.mul => "Int64.mul".
+Extract Constant Pos.min => "Pervasives.min".
+Extract Constant Pos.max => "Pervasives.max".
+Extract Constant Pos.compare =>
+ "fun x y -> if x=y then Eq else if x<y then Lt else Gt".
+Extract Constant Pos.compare_cont =>
+ "fun c x y -> if x=y then c else if x<y then Lt else Gt".
+
+
+
+Extract Inductive N => int64 [ "Int64.zero" "" ]
+"(fun f0 fp n -> if n=Int64.zero then f0 () else fp n)".
+
+Extract Constant N.add => "Int64.add".
+Extract Constant N.succ => "Int64.succ".
+Extract Constant N.pred => "fun n -> Pervasives.max Int64.zero (Int64.sub n Int64.one)".
+Extract Constant N.sub => "fun n m -> Pervasives.max Int64.zero (Int64.sub n m)".
+Extract Constant N.mul => "Int64.mul".
+Extract Constant N.min => "Pervasives.min".
+Extract Constant N.max => "Pervasives.max".
+Extract Constant N.div => "fun a b -> if b=Int64.zero then Int64.zero else (Int64.div a b)".
+Extract Constant N.modulo => "fun a b -> if b=Int64.zero then a else Int64.rem a b".
+Extract Constant N.compare =>
+ "fun x y -> if x=y then Eq else if x<y then Lt else Gt".
+
+Extract Constant N.shiftl => "fun a b -> Int64.shift_left a (Int64.to_int b)".
+Extract Constant N.shiftr => "fun a b -> Int64.shift_right_logical a (Int64.to_int b)".
+Extract Constant N.lor => "Int64.logor".
+Extract Constant N.land => "Int64.logand".
+Extract Constant N.eqb => "(=)".
+Extract Constant N.eq_dec => "(=)".
 Extract Constant N.ltb => "(<)".
-Extract Constant N.div2 => "(fun x -> x / 2)".
+Extract Constant N.div2 => "(fun x -> Int64.div x (Int64.of_int 2))".
+(* Extract Constant N.div_eucl => "(fun x y -> (Int64.div x y, Int64.rem x y))". *)
+Extract Constant Varint_split => "(fun n -> (Int64.shift_right_logical n 7, Int64.logand n 127L))".
 (* :TODO: Get rid of power and instead use bit operations *)
-Extract Constant N.pow => "Batteries.Int.pow".
+Extract Constant N.pow => "Batteries.Int64.pow".
